cava/Cava/Arrow/CavaNotation.v
@@ -24,22 +24,36 @@ From Cava Require Import Arrow.Primitives.
 Import ListNotations.
 Import EqNotations.
 
-Local Open Scope category_scope.
-Local Open Scope arrow_scope.
-
 Declare Scope kappa_scope.
 Declare Custom Entry expr.
 Delimit Scope kappa_scope with kappa.
 
+Set Implicit Arguments.
+Generalizable All Variables.
+
 (* Kappa expression and application *)
 
 Module KappaNotation.
-  Notation "<[ e ]>" := (
-    (fun var => e%kappa)
-   ) (at level 1, e custom expr at level 1).
 
-  Notation "\ x .. y => e" := (Abs (fun x => .. (Abs (fun y => e)) ..))
-    (in custom expr at level 200, x binder, right associativity) : kappa_scope.
+  Notation "<[ 'fun' name x .. y : ret => e ]>" := (
+    mkModule name (fun var =>
+      (Abs (fun x => .. (Abs (fun y => e)) ..)) : kappa var _ ret
+    %kappa)
+   ) (at level 1, name constr at level 1, x closed binder, e custom expr at level 99).
+
+  Notation "<[ \ x .. y => e ]>" := (
+    (fun var => (Abs (fun x => .. (Abs (fun y => e)) ..))%kappa): Kappa _ _
+   ) (at level 1, x closed binder, e custom expr at level 1).
+
+  Notation "<[ \ x .. y : ret => e ]>" := (
+    (fun var => (Abs (fun x => .. (Abs (fun y => e)) ..))%kappa): Kappa _ ret
+   ) (at level 1, x closed binder, e custom expr at level 1).
+
+  Notation "<[ e ]>" := (
+    (fun var => (e)%kappa): Kappa _ _
+   ) (at level 1, e custom expr at level 99).
+
+  Notation "x ~> y" := (Kappa x y) (at level 90).
 
   Notation "x y" := (App x y) (in custom expr at level 3, left associativity) : kappa_scope.
 
@@ -52,145 +66,27 @@ Module KappaNotation.
   Notation "'letrec' x = a 'in' b" := (LetRec (fun x => a) (fun x => b))
     (in custom expr at level 1, x constr at level 4, b at level 7, a at level 1) : kappa_scope.
 
-  (* TODO(blaxill): can this be turned into a recursive pattern?
-  The binders not mentioned on the lhs (e.g. a_binder) prevent me from doing this
-  I think. Moving away from PHOAS would also work *)
+  (* destructuring *)
+  Notation "'let' '( x , .. , y ) : ty = a 'in' e" := (
+    Let (a : kappa _ Unit ty) (fun a_var => Comp1
+      (Abs (fun x => .. (Abs (fun y => e)) ..) )
+      (Var a_var : kappa _ Unit ty)
+    ) )
+    ( in custom expr at level 1, x closed binder, ty constr at level 7, e at level 7) : kappa_scope.
 
-  (* This function shouldn't be necessary but helps with type unification when
-  using the tuple destructuring notation *)
-  Definition proj1_tuple1 ty: CircuitPrimitive :=
-    match ty with
-    | Tuple l r => Fst l r
-    | _ => Fst Unit Unit
-    end.
-
-  Notation "'let' '( x , y ) = a 'in' b" := (
-    Let a (fun a_binder =>
-    Let (App (Primitive (Fst _ _)) (Var a_binder)) (fun x =>
-      Let (App (Primitive (Snd _ _)) (Var a_binder)) (fun y => b))))
-    ( in custom expr at level 1, x constr, y constr, b at level 7) : kappa_scope.
-
-  Notation "'let' '( x , y ) : ty = a 'in' b" := (
-    Let a (fun a_binder =>
-    Let (App (Primitive (proj1_tuple1 ty)) (Var a_binder)) (fun x =>
-      Let (App (Primitive (Snd _ _ )) (Var a_binder)) (fun y => b))))
-    ( in custom expr at level 1, x constr, y constr, ty constr at level 7, b at level 7) : kappa_scope.
-
-  Notation "'let' '( x , y , z ) = a 'in' b" := (
-    Let a (fun a_binder =>
-    Let (App (Primitive (Fst _ _ )) (Var a_binder)) (fun x =>
-      Let (App (Primitive (Snd _ _ )) (Var a_binder)) (fun a_tl_binder =>
-        Let (App (Primitive (Fst _ _ )) (Var a_tl_binder)) (fun y =>
-          Let (App (Primitive (Snd _ _ )) (Var a_tl_binder)) (fun z =>
-          b))))))
-    ( in custom expr at level 1, x constr, y constr, z constr, b at level 7) : kappa_scope.
-  Notation "'let' '( x , y , z , w ) = a 'in' b" := (
-    Let a (fun a_binder =>
-    Let (App (Primitive (Fst _ _ )) (Var a_binder)) (fun x =>
-      Let (App (Primitive (Snd _ _ )) (Var a_binder)) (fun a_tl_binder =>
-        Let (App (Primitive (Fst _ _ )) (Var a_tl_binder)) (fun y =>
-            Let (App (Primitive (Snd _ _ )) (Var a_tl_binder)) (fun a_tl_tl_binder =>
-              Let (App (Primitive (Fst _ _ )) (Var a_tl_tl_binder)) (fun z =>
-                Let (App (Primitive (Snd _ _ )) (Var a_tl_tl_binder)) (fun w =>
-          b))))))))
-    ( in custom expr at level 1, x constr, y constr, z constr, w constr, b at level 7) : kappa_scope.
-  Notation "'let' '( x1 , x2 , x3 , x4 , x5 ) = a 'in' b" := (
-    Let a (fun binder1 =>
-    Let (App (Primitive (Fst _ _ )) (Var binder1)) (fun x1 =>
-      Let (App (Primitive (Snd _ _ )) (Var binder1)) (fun binder2 =>
-        Let (App (Primitive (Fst _ _ )) (Var binder2)) (fun x2 =>
-            Let (App (Primitive (Snd _ _ )) (Var binder2)) (fun binder3 =>
-              Let (App (Primitive (Fst _ _ )) (Var binder3)) (fun x3 =>
-                Let (App (Primitive (Snd _ _ )) (Var binder3)) (fun binder4 =>
-                  Let (App (Primitive (Fst _ _ )) (Var binder4)) (fun x4 =>
-                    Let (App (Primitive (Snd _ _ )) (Var binder4)) (fun x5 =>
-          b))))))))))
-    ( in custom expr at level 1
-    , x1 constr, x2 constr, x3 constr, x4 constr, x5 constr
-    , b at level 7) : kappa_scope.
-  Notation "'let' '( x1 , x2 , x3 , x4 , x5 , x6 ) = a 'in' b" := (
-    Let a (fun binder1 =>
-    Let (App (Primitive (Fst _ _ )) (Var binder1)) (fun x1 =>
-      Let (App (Primitive (Snd _ _ )) (Var binder1)) (fun binder2 =>
-        Let (App (Primitive (Fst _ _ )) (Var binder2)) (fun x2 =>
-            Let (App (Primitive (Snd _ _ )) (Var binder2)) (fun binder3 =>
-              Let (App (Primitive (Fst _ _ )) (Var binder3)) (fun x3 =>
-                Let (App (Primitive (Snd _ _ )) (Var binder3)) (fun binder4 =>
-                  Let (App (Primitive (Fst _ _ )) (Var binder4)) (fun x4 =>
-                    Let (App (Primitive (Snd _ _ )) (Var binder4)) (fun binder5 =>
-                      Let (App (Primitive (Fst _ _ )) (Var binder5)) (fun x5 =>
-                        Let (App (Primitive (Snd _ _ )) (Var binder5)) (fun x6 =>
-          b))))))))))))
-    ( in custom expr at level 1
-    , x1 constr, x2 constr, x3 constr, x4 constr, x5 constr, x6 constr
-    , b at level 7) : kappa_scope.
-  Notation "'let' '( x1 , x2 , x3 , x4 , x5 , x6 , x7 ) = a 'in' b" := (
-    Let a (fun binder1 =>
-    Let (App (Primitive (Fst _ _ )) (Var binder1)) (fun x1 =>
-      Let (App (Primitive (Snd _ _ )) (Var binder1)) (fun binder2 =>
-        Let (App (Primitive (Fst _ _ )) (Var binder2)) (fun x2 =>
-            Let (App (Primitive (Snd _ _ )) (Var binder2)) (fun binder3 =>
-              Let (App (Primitive (Fst _ _ )) (Var binder3)) (fun x3 =>
-                Let (App (Primitive (Snd _ _ )) (Var binder3)) (fun binder4 =>
-                  Let (App (Primitive (Fst _ _ )) (Var binder4)) (fun x4 =>
-                    Let (App (Primitive (Snd _ _ )) (Var binder4)) (fun binder5 =>
-                      Let (App (Primitive (Fst _ _ )) (Var binder5)) (fun x5 =>
-                        Let (App (Primitive (Snd _ _ )) (Var binder5)) (fun binder6 =>
-                            Let (App (Primitive (Fst _ _ )) (Var binder6)) (fun x6 =>
-                              Let (App (Primitive (Snd _ _ )) (Var binder6)) (fun x7 =>
-          b))))))))))))))
-    ( in custom expr at level 1
-    , x1 constr, x2 constr, x3 constr, x4 constr, x5 constr, x6 constr, x7 constr
-    , b at level 7) : kappa_scope.
-
-  Notation "'let' '( x1 , x2 , x3 , x4 , x5 , x6 , x7 ) : ty = a 'in' b" := (
-    Let a (fun binder1 =>
-    Let (App (Primitive (proj1_tuple1 ty)) (Var binder1)) (fun x1 =>
-      Let (App (Primitive (Snd _ _ )) (Var binder1)) (fun binder2 =>
-        Let (App (Primitive (Fst _ _ )) (Var binder2)) (fun x2 =>
-            Let (App (Primitive (Snd _ _ )) (Var binder2)) (fun binder3 =>
-              Let (App (Primitive (Fst _ _ )) (Var binder3)) (fun x3 =>
-                Let (App (Primitive (Snd _ _ )) (Var binder3)) (fun binder4 =>
-                  Let (App (Primitive (Fst _ _ )) (Var binder4)) (fun x4 =>
-                    Let (App (Primitive (Snd _ _ )) (Var binder4)) (fun binder5 =>
-                      Let (App (Primitive (Fst _ _ )) (Var binder5)) (fun x5 =>
-                        Let (App (Primitive (Snd _ _ )) (Var binder5)) (fun binder6 =>
-                            Let (App (Primitive (Fst _ _ )) (Var binder6)) (fun x6 =>
-                              Let (App (Primitive (Snd _ _ )) (Var binder6)) (fun x7 =>
-          b))))))))))))))
-    ( in custom expr at level 1
-    , x1 constr, x2 constr, x3 constr, x4 constr, x5 constr, x6 constr, x7 constr
-    , ty constr at level 7
-    , b at level 7) : kappa_scope.
-
-  Notation "'let' '( x1 , x2 , x3 , x4 , x5 , x6 , x7 , x8 ) : ty = a 'in' b" := (
-    Let a (fun binder1 =>
-    Let (App (Primitive (proj1_tuple1 ty)) (Var binder1)) (fun x1 =>
-      Let (App (Primitive (Snd _ _ )) (Var binder1)) (fun binder2 =>
-        Let (App (Primitive (Fst _ _ )) (Var binder2)) (fun x2 =>
-            Let (App (Primitive (Snd _ _ )) (Var binder2)) (fun binder3 =>
-              Let (App (Primitive (Fst _ _ )) (Var binder3)) (fun x3 =>
-                Let (App (Primitive (Snd _ _ )) (Var binder3)) (fun binder4 =>
-                  Let (App (Primitive (Fst _ _ )) (Var binder4)) (fun x4 =>
-                    Let (App (Primitive (Snd _ _ )) (Var binder4)) (fun binder5 =>
-                      Let (App (Primitive (Fst _ _ )) (Var binder5)) (fun x5 =>
-                        Let (App (Primitive (Snd _ _ )) (Var binder5)) (fun binder6 =>
-                            Let (App (Primitive (Fst _ _ )) (Var binder6)) (fun x6 =>
-                              Let (App (Primitive (Snd _ _ )) (Var binder6)) (fun binder7 =>
-                                  Let (App (Primitive (Fst _ _ )) (Var binder7)) (fun x7 =>
-                                    Let (App (Primitive (Snd _ _ )) (Var binder7)) (fun x8 =>
-          b))))))))))))))))
-    ( in custom expr at level 1
-    , x1 constr, x2 constr, x3 constr, x4 constr, x5 constr, x6 constr, x7 constr, x8 constr
-    , ty constr at level 7
-    , b at level 7) : kappa_scope.
+  Notation "'let' '( x , .. , y ) = a 'in' e" := (
+    Let a (fun a_var => Comp1
+      (Abs (fun x => .. (Abs (fun y => e)) ..) )
+      (Var a_var )
+    ) )
+    ( in custom expr at level 1, x closed binder, e at level 7) : kappa_scope.
 
   (* Escaping *)
 
   Notation "! x" := (RemoveContext (x _))(in custom expr at level 2, x global) : kappa_scope.
   Notation "!( x )" := (RemoveContext (x _)) (in custom expr, x constr) : kappa_scope.
 
-  Notation tupleHelper := (fun x y => App (App (Primitive (Pair _ _)) x) y).
+  Notation tupleHelper := (fun x y => App (App (Primitive (P2 (Pair _ _))) x) y).
   Notation "( x , .. , y , z )" := (
     (tupleHelper x .. (tupleHelper y z) .. )
     )
@@ -198,24 +94,26 @@ Module KappaNotation.
 
   (* Pre defined functions *)
 
-  Notation "'fst'" := (Primitive (Fst _ _ )) (in custom expr at level 4) : kappa_scope.
-  Notation "'snd'" := (Primitive (Snd _ _ )) (in custom expr at level 4) : kappa_scope.
+  Notation "'typecast'" := (Typecast _ _) (in custom expr at level 4) : kappa_scope.
 
-  Notation "'not'" := (Primitive Not) (in custom expr at level 4) : kappa_scope.
-  Notation "'and'" := (Primitive And) (in custom expr at level 4) : kappa_scope.
-  Notation "'nand'" := (Primitive Nand) (in custom expr at level 4) : kappa_scope.
-  Notation "'or'" := (Primitive Or) (in custom expr at level 4) : kappa_scope.
-  Notation "'nor'" := (Primitive Nor) (in custom expr at level 4) : kappa_scope.
-  Notation "'xor'" := (Primitive Xor) (in custom expr at level 4) : kappa_scope.
-  Notation "'xnor'" := (Primitive Xnor) (in custom expr at level 4) : kappa_scope.
-  Notation "'buf'" := (Primitive BufGate) (in custom expr at level 4) : kappa_scope.
-  Notation "'delay'" := (Primitive (Delay _)) (in custom expr at level 4) : kappa_scope.
+  Notation "'fst'" := (Primitive (P1 (Fst _ _ ))) (in custom expr at level 4) : kappa_scope.
+  Notation "'snd'" := (Primitive (P1 (Snd _ _ ))) (in custom expr at level 4) : kappa_scope.
 
-  Notation "'xorcy'" := (Primitive Xorcy) (in custom expr at level 4) : kappa_scope.
-  Notation "'muxcy'" := (Primitive Muxcy) (in custom expr at level 4) : kappa_scope.
+  Notation "'not'" := (Primitive (P1 Not)) (in custom expr at level 4) : kappa_scope.
+  Notation "'and'" := (Primitive (P2 And)) (in custom expr at level 4) : kappa_scope.
+  Notation "'nand'" := (Primitive (P2 Nand)) (in custom expr at level 4) : kappa_scope.
+  Notation "'or'" := (Primitive (P2 Or)) (in custom expr at level 4) : kappa_scope.
+  Notation "'nor'" := (Primitive (P2 Nor)) (in custom expr at level 4) : kappa_scope.
+  Notation "'xor'" := (Primitive (P2 Xor)) (in custom expr at level 4) : kappa_scope.
+  Notation "'xnor'" := (Primitive (P2 Xnor)) (in custom expr at level 4) : kappa_scope.
+  Notation "'buf'" := (Primitive (P1 BufGate)) (in custom expr at level 4) : kappa_scope.
+  Notation "'delay'" := (ExprSyntax.Delay) (in custom expr at level 4) : kappa_scope.
 
-  Definition unsigned_add2 {var a b} := Primitive (var:=var) (UnsignedAdd a b (S (max a b))).
-  Definition unsigned_add1 {var a} := Primitive (var:=var) (UnsignedAdd a a a).
+  Notation "'xorcy'" := (Primitive (P2 Xorcy)) (in custom expr at level 4) : kappa_scope.
+  Notation "'muxcy'" := (Primitive (P2 Muxcy)) (in custom expr at level 4) : kappa_scope.
+
+  Definition unsigned_add2 {var a b} := Primitive (var:=var) (P2 (UnsignedAdd a b (S (max a b)))).
+  Definition unsigned_add1 {var a} := Primitive (var:=var) (P2 (UnsignedAdd a a a)).
 
   Notation "x + y" :=
       (App (App unsigned_add2 x) y)
@@ -223,26 +121,26 @@ Module KappaNotation.
   Notation "x +% y" :=
       (App (App unsigned_add1 x) y)
       (in custom expr at level 4) : kappa_scope.
-  Notation "x - y" := (App (App ((Primitive (UnsignedSub _))) x) y) (in custom expr at level 4) : kappa_scope.
-  Notation "'unsigned_add' a b c" := ((Primitive (UnsignedAdd a b c)))
+  Notation "x - y" := (App (App ((Primitive (P2 (UnsignedSub _)))) x) y) (in custom expr at level 4) : kappa_scope.
+  Notation "'unsigned_add' a b c" := ((Primitive (P2 (UnsignedAdd a b c))))
     (in custom expr at level 4,
     a constr at level 4,
     b constr at level 4,
     c constr at level 4
     ) : kappa_scope.
-  Notation "'unsigned_sub' a" := ((Primitive (UnsignedSub a)))
+  Notation "'unsigned_sub' a" := ((Primitive (P2 (UnsignedSub a))))
     (in custom expr at level 4,
     a constr at level 4
     ) : kappa_scope.
 
-  Notation "'[]'" := ((Primitive (EmptyVec _))) (in custom expr at level 4) : kappa_scope.
-  Notation "x ++ y" := (App (App ((Primitive (Concat _ _))) x) y) (in custom expr at level 4) : kappa_scope.
-  Notation "x :: y" := (App (App ((Primitive (Cons _ _))) x) y) (in custom expr at level 7, right associativity) : kappa_scope.
+  Notation "'[]'" := (Primitive (P0 (EmptyVec _))) (in custom expr at level 4) : kappa_scope.
+  Notation "x ++ y" := (App (App (Primitive (P2 (Concat _ _))) x) y) (in custom expr at level 4) : kappa_scope.
+  Notation "x :: y" := (App (App (Primitive (P2 (Cons _ _))) x) y) (in custom expr at level 7, right associativity) : kappa_scope.
 
-  Notation "'true''" := ((Primitive (Constant Bit true))) (in custom expr at level 2) : kappa_scope.
-  Notation "'false''" := ((Primitive (Constant Bit false))) (in custom expr at level 2) : kappa_scope.
+  Notation "'true''" := (Primitive (P0 (Constant Bit true))) (in custom expr at level 2) : kappa_scope.
+  Notation "'false''" := (Primitive (P0 (Constant Bit false))) (in custom expr at level 2) : kappa_scope.
 
-  Notation "# x" := ((Primitive (Constant (Vector Bit _) (N2Bv_sized _ x))))%N
+  Notation "# x" := (Primitive (P0 (Constant (Vector Bit _) (N2Bv_sized _ x))))%N
     (in custom expr at level 2,
     x constr at level 4, no associativity) : kappa_scope.
 
@@ -250,87 +148,86 @@ Module KappaNotation.
   Notation "{ x , y , .. , z }" :=
     (
       let ls := (cons x (cons y .. (cons z nil) ..)) in
-      (Primitive
+      (Primitive (P0
       (ConstantVec
         (List.length ls)
         (Vector Bit _)
         (List.map (N2Bv_sized _) ls)
-      )))%list%N
+      ))))%list%N
     (in custom expr at level 2,
     x constr at level 4, y constr at level 4, z constr at level 4, no associativity) : kappa_scope.
 
-  Notation "v [ x ]" := (App (App ((Primitive (Index _ _))) v) x)
+  Notation "v [ x ]" := (App (App (Primitive (P2 (Index _ _))) v) x)
     ( in custom expr at level 2
     , x at level 7
     ) : kappa_scope.
   Notation "v [: x : y ]" :=
-        (App ((Primitive (Slice _ (x <: nat) (y <: nat) _))) v)
+        (App (Primitive (P1 (Slice _ (x <: nat) (y <: nat) _))) v)
     (in custom expr at level 2,
     (* v constr, *)
     x constr at level 7,
     y constr at level 7
     ) : kappa_scope.
 
-  Notation "'index'" := ((Primitive (Index _ _))) (in custom expr at level 4) : kappa_scope.
-  Notation "'empty'" := ((Primitive EmptyVec)) (in custom expr at level 4) : kappa_scope.
-  Notation "'cons'" := ((Primitive (Cons _ _))) (in custom expr at level 4) : kappa_scope.
-  Notation "'snoc'" := ((Primitive (Snoc _ _))) (in custom expr at level 4) : kappa_scope.
-  Notation "'concat'" := ((Primitive (Concat _ _ _))) (in custom expr at level 4) : kappa_scope.
-  Notation "'split_at' x" := ((Primitive (Split x _ _))) (in custom expr at level 4, x constr at level 4) : kappa_scope.
-  Notation "'uncons'" := ((Primitive (Uncons _ _))) (in custom expr at level 4) : kappa_scope.
-  Notation "'unsnoc'" := ((Primitive (Unsnoc _ _))) (in custom expr at level 4) : kappa_scope.
+  Notation "'index'" := (Primitive (P2 (Index _ _))) (in custom expr at level 4) : kappa_scope.
+  Notation "'empty'" := (Primitive (P0 EmptyVec)) (in custom expr at level 4) : kappa_scope.
+  Notation "'cons'" := (Primitive (P2 (Cons _ _))) (in custom expr at level 4) : kappa_scope.
+  Notation "'snoc'" := (Primitive (P2 (Snoc _ _))) (in custom expr at level 4) : kappa_scope.
+  Notation "'concat'" := (Primitive (P2 (Concat _ _ _))) (in custom expr at level 4) : kappa_scope.
+  Notation "'split_at' x" := (Primitive (P1 (Split x _ _))) (in custom expr at level 4, x constr at level 4) : kappa_scope.
+  Notation "'uncons'" := (Primitive (P1 (Uncons _ _))) (in custom expr at level 4) : kappa_scope.
+  Notation "'unsnoc'" := (Primitive (P1 (Unsnoc _ _))) (in custom expr at level 4) : kappa_scope.
 
 End KappaNotation.
-
-Import KappaNotation.
-Local Open Scope kind_scope.
 
 Section regression_examples.
   Import KappaNotation.
   Local Open Scope kappa_scope.
 
-  Definition ex0_constant:  << Vector Bit 10, Unit >> ~[KappaCat]~> (Vector Bit 8)
-    := <[ \x => x [: 7 : 0 ] ]>.
+  Definition ex0_constant
+    := <[ fun "ex0_constant" ( x : _ (Vector Bit 8) ) : Vector Bit 8 => x [: 7 : 0 ] ]>.
 
+  Definition ex1_constant: Kappa << Bit, Unit >> Bit := <[ \ x => true' ]> .
 
-  Definition ex1_constant:  << Bit, Unit >> ~> Bit := <[ \x => true' ]>.
-  Definition ex2_parameterized (n: nat):  << Bit, Unit >> ~> Bit :=
+  Definition ex2_parameterized (n: nat): Kappa << Bit, Unit >> Bit :=
   match n with
-  | O => <[ \ x => true' ]>
-  | S n => <[ \ x => xor x x ]>
+  | O => <[\x => true' ]>
+  | S n => <[\x => xor x x ]>
   end.
 
-  Definition ex3_to_vec:  << Bit, Unit >> ~> (Vector Bit 1) :=
+  Definition ex3_to_vec: Kappa << Bit, Unit >> (Vector Bit 1) :=
   <[ \ x => x :: [] ]>.
-  Definition ex4_index_vec:  << Vector Bit 10, Unit >> ~> Bit :=
+  Definition ex4_index_vec:  Kappa << Vector Bit 10, Unit >> Bit :=
   <[ \ x => index x (# 1) ]>.
-  Definition ex5_index_vec2:  << Vector Bit 10, Unit >> ~> Bit :=
+  Definition ex5_index_vec2:  Kappa << Vector Bit 10, Unit >> Bit :=
   <[ \ x => x [# 1] ]>.
-  Definition ex6_concat:  << Vector Bit 2, Bit, Unit >> ~> (Vector Bit 3) :=
+  Definition ex6_concat:  Kappa << Vector Bit 2, Bit, Unit >> (Vector Bit 3) :=
   <[ \ x v => snoc x v ]>.
-  Definition ex7_xor:  << Bit, Bit, Unit >> ~> Bit :=
-  <[ \ x y => xor x y ]>.
-  Definition ex7_tupled_destruct:  << << Bit, Bit>>, Unit>> ~> Bit :=
+
+  Definition ex7_xor :=
+    <[fun "ex7_xor" (x : _ Bit) (y : _ Bit) : Bit => xor x y ]>.
+
+  Definition ex7_tupled_destruct:  Kappa << << Bit, Bit>>, Unit>> Bit :=
   <[ \ xy =>
     let '(x,y) : <<Bit,Bit>> = xy in
     y ]>.
-  Definition ex8_multiindex:  << Vector (Vector Bit 5) 10, Unit >> ~> Bit :=
+  Definition ex8_multiindex:  Kappa << Vector (Vector Bit 5) 10, Unit >> Bit :=
   <[ \ x => x[#0][#1] ]>.
-  Definition ex9_mkvec:  << Bit, Unit >> ~> (Vector Bit 2) :=
+  Definition ex9_mkvec:  Kappa << Bit, Unit >> (Vector Bit 2) :=
   <[ \x => true' :: false' :: [] ]>.
-  Definition ex10:  << Vector Bit 10, Vector Bit 10, Unit >> ~> (Vector Bit 11) :=
+  Definition ex10:  Kappa << Vector Bit 10, Vector Bit 10, Unit >> (Vector Bit 11) :=
   <[ \ x y => x + y ]>.
-  Definition ex11:  << Vector Bit 10, Vector Bit 10, Unit >> ~> (Vector Bit 10) :=
+  Definition ex11:  Kappa << Vector Bit 10, Vector Bit 10, Unit >> (Vector Bit 10) :=
   <[ \ x y => x +% y ]>.
-  Definition ex13:  << Vector Bit 10, Unit >> ~> Bit :=
+  Definition ex13:  Kappa << Vector Bit 10, Unit >> Bit :=
   <[ \ x => (xor x[#0] x[#1] :: false' :: []) [#0] ]>.
-  Definition ex14:  << Vector Bit 10, Vector Bit 4, Unit >> ~> Bit :=
+  Definition ex14:  Kappa << Vector Bit 10, Vector Bit 4, Unit >> Bit :=
   <[ \ x i => x [ i ] ]>.
-  Definition ex15_rec_xor:  << Bit, Unit >> ~> Bit :=
+  Definition ex15_rec_xor:  Kappa << Bit, Unit >> Bit :=
   <[ \ x => letrec s = delay (xor x s) in s ]>.
-  Definition ex16_triple:  << <<Bit, Bit, Bit>>, Unit >> ~> Bit :=
-  <[ \ triple => let '(x, y, z) = triple in x ]>.
-  Definition ex17_constant_via_list:  << Unit >> ~> Vector (Vector Bit 4) 3 := <[  { 1, 2, 3 } ]>.
+  Definition ex16_triple:  Kappa << <<Bit, Bit, Bit>>, Unit >> Bit :=
+  <[ \ triple => let '(x, y, z) : <<Bit,Bit,Bit>> = triple in x ]>.
+  Definition ex17_constant_via_list: Kappa << Unit >> (Vector (Vector Bit 4) 3) := <[ { 1, 2, 3 } ]>.
 
   Fixpoint copy_object_pow2 o (n:nat): Kind :=
   match n with
@@ -338,29 +235,30 @@ Section regression_examples.
   | S n => Tuple (copy_object_pow2 o n) (copy_object_pow2 o n)
   end.
 
-  Program Fixpoint tree
+  Fixpoint tree
     (A: Kind)
     (n: nat)
     (f: << A, A, Unit >> ~> A)
     {struct n}
-    :  << copy_object_pow2 A n, Unit >> ~> A :=
+    : Kappa << copy_object_pow2 A n, Unit >> A :=
   match n with
-  | O => <[ \ x => x ]>
+  | O =>
+    <[ \ x => x ]>
   | S n' =>
     <[\ x =>
-        let a = !(tree A n' f) (fst x) in
-        let b = !(tree A n' f) (snd x) in
+        let a = !(tree n' f) (fst x) in
+        let b = !(tree n' f) (snd x) in
         !f a b
     ]>
   end.
 
   Definition adder_tree
     (bitsize n: nat)
-    : <<copy_object_pow2 (Vector Bit bitsize) n, Unit>> ~> (Vector Bit bitsize) :=
-    tree (Vector Bit bitsize) n <[\x y => x +% y]>.
+    : Kappa <<copy_object_pow2 (Vector Bit bitsize) n, Unit>> (Vector Bit bitsize) :=
+    <[ !(tree n <[\x y => x +% y]> ) ]>.
 
   Definition xilinxFullAdder
-    :  << Bit, << Bit, Bit >>, Unit>> ~> (Tuple Bit Bit) :=
+    : Kappa << Bit, << Bit, Bit >>, Unit>> (Tuple Bit Bit) :=
     <[ \ cin ab =>
       let a = fst ab in
       let b = snd ab in
@@ -371,27 +269,28 @@ Section regression_examples.
     ]>.
 
   Fixpoint reshape {n m A}
-    :  << Vector A (n * m), Unit >> ~> << Vector (Vector A m) n >> :=
+    : Kappa << Vector A (n * m), Unit >> << Vector (Vector A m) n >> :=
   match n with
   | 0 => <[\_ => [] ]>
   | S n' =>
     <[ \vec =>
-      let '(x, xs) = split_at m vec in
+      let '(x, xs) : <<Vector A _, Vector A _>> = split_at m vec in
       x :: !(@reshape n' m A) xs
       ]>
   end.
 
   Definition dummy {T}
-    :  << Bit, T, T, Unit >> ~> <<T>> :=
+    : Kappa << Bit, T, T, Unit >> <<T>> :=
     <[\_ x _ => x]>.
   Notation T:=(Bit )(only parsing).
   Notation "'if' i 'then' t 'else' e" :=
     (App (App (App (dummy _) i) t) e)
     (in custom expr at level 5, left associativity) : kappa_scope.
-  Definition exfailed: << <<T,T>>,<<T,T>>, Unit >> ~> <<T,T>> :=
+
+  Definition exfailed: Kappa << <<T,T>>,<<T,T>>, Unit >> <<T,T>> :=
     <[\s1 s2 =>
     let '(a,b) : <<_,T>> =  s1 in
-    let '(aa,bb) : <<_,_>> = s2 in
+    let '(aa,bb) : <<_,T>> = s2 in
     if a then (a,b) else s1
     ]>.
 
