cava/Cava/Arrow/ExprEquiv.v
@@ -42,6 +42,13 @@ Set Asymmetric Patterns.
       -> kappa_equivalence E g1 g2
       -> kappa_equivalence E (Comp f1 g1) (Comp f2 g2)
 
+    | Compose1_equiv : forall E x y z
+      (f1: kappa var1 y z) (f2: kappa var2 y z)
+      (g1: kappa var1 x (remove_rightmost_unit y)) (g2: kappa var2 x (remove_rightmost_unit y)),
+      kappa_equivalence E f1 f2
+      -> kappa_equivalence E g1 g2
+      -> kappa_equivalence E (Comp1 f1 g1) (Comp1 f2 g2)
+
     | Prim_equiv : forall E p, kappa_equivalence E (ExprSyntax.Primitive p) (ExprSyntax.Primitive p)
 
     | Let_equiv : forall x y z
@@ -69,6 +76,9 @@ Set Asymmetric Patterns.
       kappa_equivalence E (LetRec v1 f1) (LetRec v2 f2)
 
     | Id_equiv : forall x E, kappa_equivalence E (@Id var1 x) Id
+    | Typecast_equiv : forall x y E, kappa_equivalence E (@Typecast var1 x y) (Typecast x y)
+
+    | Delay_equiv : forall x E, kappa_equivalence E (@Delay var1 x) Delay
 
     | RemoveContext_equiv : forall x y E
       (f1 : kappa var1 x y)
@@ -76,6 +86,13 @@ Set Asymmetric Patterns.
       kappa_equivalence nil f1 f2
       ->
       kappa_equivalence E (RemoveContext f1) (RemoveContext f2)
+
+    | CallModule_equiv : forall x y E
+      (f1 : Module (kappa var1 x y))
+      (f2 : Module (kappa var2 x y)),
+      kappa_equivalence nil (module_body f1) (module_body f2)
+      ->
+      kappa_equivalence E (CallModule f1) (CallModule f2)
     .
 
   End Equivalence.
