cava/Cava/Arrow/ExprSyntax.v
@@ -1,3 +1,4 @@
+From Coq Require Import Strings.String.
 From Coq Require Import Lists.List.
 From Coq Require Import Arith.Peano_dec.
 From Cava Require Import Arrow.ArrowKind.
@@ -13,6 +14,23 @@ Section vars.
   Definition natvar : Kind -> Type := fun _ => nat.
   Definition unitvar : Kind -> Type := fun _ => unit.
 
+  Definition extended_prim_input p :=
+    match p with
+    | P0 _ _ => Unit
+    | P1 x _ _ => Tuple x Unit
+    | P2 x y z _ => Tuple x (Tuple y Unit)
+    end.
+
+  Record Module ( body_ty : Type ) := mkModule
+    { module_name : string
+    ; module_body : body_ty
+    }.
+
+  Definition module_map_body {A B} (m: Module A) (f: A -> B): Module B :=
+    match m with
+    | mkModule name body => mkModule name (f body)
+    end.
+
   Section Vars.
     Variable (var: Kind -> Type).
 
@@ -21,11 +39,15 @@ Section vars.
     | Abs : forall {x y z}, (var x -> kappa y z) -> kappa (Tuple x y) z
     | App : forall {x y z}, kappa (Tuple x y) z -> kappa Unit x -> kappa y z
     | Comp: forall {x y z}, kappa y z -> kappa x y -> kappa x z
-    | Primitive : forall prim, kappa (primitive_input prim) (primitive_output prim)
+    | Comp1: forall {x y z}, kappa y z -> kappa x (remove_rightmost_unit y) -> kappa x z
+    | Delay: forall {x}, kappa (Tuple x Unit) x
+    | Primitive : forall prim, kappa (extended_prim_input prim) (primitive_output prim)
     | Let: forall {x y z}, kappa Unit x -> (var x -> kappa y z) -> kappa y z
     | LetRec : forall {x y z}, (var x -> kappa Unit x) -> (var x -> kappa y z) -> kappa y z
     | Id : forall {x}, kappa x x
+    | Typecast : forall x y, kappa (Tuple x Unit) y
     | RemoveContext: forall {x y}, kappa x y -> kappa x y
+    | CallModule: forall {x y}, Module (kappa x y) -> kappa x y
     .
   End Vars.
 
@@ -50,24 +72,39 @@ Section vars.
     | Abs x _ _ f => wf_phoas_context (x :: ctxt) (f (length ctxt))
     | App _ _ _ e1 e2 => wf_phoas_context ctxt e1 /\ wf_phoas_context ctxt e2
     | Comp _ _ _ e1 e2 => wf_phoas_context ctxt e1 /\ wf_phoas_context ctxt e2
+    | Comp1 _ _ _ e1 e2 => wf_phoas_context ctxt e1 /\ wf_phoas_context ctxt e2
+    | Delay _ => True
     | Primitive _ => True
     | Id _ => True
+    | Typecast x y => True
     | Let x _ _ v f => wf_phoas_context (x :: ctxt) (f (length ctxt)) /\ wf_phoas_context ctxt v
     | LetRec x _ _ v f => wf_phoas_context (x :: ctxt) (v (length ctxt)) /\ wf_phoas_context (x :: ctxt) (f (length ctxt))
     | RemoveContext _ _ f => wf_phoas_context [] f
+    | CallModule _ _ (mkModule _ m) => wf_phoas_context [] m
     end.
 
   Definition Kappa i o := forall var, kappa var i o.
 
+  Definition module_instantiate_var {var x y} (m: Module (Kappa x y)): Module (kappa var x y) :=
+    module_map_body m (fun e => e var).
+  Definition module_to_expr {x y} (e: Module (Kappa x y)): Kappa x y :=
+    fun var => CallModule (module_instantiate_var e).
+
+  Coercion module_to_expr: Module >-> Kappa.
 End vars.
 
 Arguments Var {var _}.
 Arguments Abs {var _ _ _}.
 Arguments App {var _ _ _}.
 Arguments Comp {var _ _ _}.
+Arguments Comp1 {var _ _ _}.
+Arguments Delay {var _}.
 Arguments Primitive {var}.
 Arguments LetRec {var _ _ _}.
 Arguments Id {var _}.
+Arguments Typecast {var}.
+Arguments RemoveContext {var _ _}.
+Arguments CallModule {var _ _}.
 
 Instance KappaCat : Category Kind := {
   morphism X Y := forall var, kappa var X Y;
